NIProof.v
@@ -463,13 +463,7 @@ by apply/(flows_trans _ _ _ low_lv); rewrite flows_join low_lv' low_lf.
     by rewrite in_regs_f1.
   by rewrite in_stack_f1 orbT.
 (* BNZ *)
-+ move=> im μ σ pc n m K r r1 j LPC rpcl -> ? get_r1 [<-] _ wf_st l f1 f2.
-  rewrite /Vector.nth_order /= root_set_registers_join !inE.
-  case/orP=> [/andP [_ in_regs_f1]|in_stack_f1]; apply: wf_st; rewrite inE.
-    by rewrite in_regs_f1.
-  by rewrite in_stack_f1 orbT.
-(* BNZ *)
-  + move=> im μ σ pc n m K r r1 j LPC rpcl -> ? get_r1 [<-] _ wf_st l f1 f2.
++ move=> im μ σ pc n m K r r1 j LPC rpcl -> ? get_r1 [<-] wf_st l f1 f2.
   rewrite /Vector.nth_order /= root_set_registers_join !inE.
   case/orP=> [/andP [_ in_regs_f1]|in_stack_f1]; apply: wf_st; rewrite inE.
     by rewrite in_regs_f1.
@@ -803,9 +797,6 @@ constructor=> [obs s1 s2 s1' s2' wf_s1 wf_s2 low_pc indist_s1s2 /fstepP step1|o 
 (* BNZ *)
 + move=> im μ σ pc n m K r r1 j LPC rpcl -> ? get_r1 [<-] ?.
   admit.
-(* BNZ *)
-  + move=> im μ σ pc n m K r r1 j LPC rpcl -> ? get_r1 [<-] ?.
-    admit.
   (* PSetOff *)
   + move=> im μ σ pc fp' j K1 n K2 r r' r1 r2 r3 j' LPC rl rpcl -> ? get_r1 get_r2 [<- <-].
     rewrite /Vector.nth_order /= => upd_r3.
@@ -887,9 +878,6 @@ constructor=> [obs s1 s2 s1' s2' wf_s1 wf_s2 low_pc indist_s1s2 /fstepP step1|o 
 (* BNZ *)
 + move=> im μ σ pc n m K r r1 j LPC rpcl -> ? get_r1 [<-] ?.
   admit.
-(* BNZ *)
-  + move=> im μ σ pc n m K r r1 j LPC rpcl -> ? get_r1 [<-] ?.
-    admit.
   (* PSetOff *)
   + move=> im μ σ pc fp' j K1 n K2 r r' r1 r2 r3 j' LPC rl rpcl -> ? get_r1 get_r2 [<- <-].
     rewrite /Vector.nth_order /= => upd_r3.
@@ -971,9 +959,6 @@ constructor=> [obs s1 s2 s1' s2' wf_s1 wf_s2 low_pc indist_s1s2 /fstepP step1|o 
 (* BNZ *)
 + move=> im μ σ pc n m K r r1 j LPC rpcl -> ? get_r1 [<-] ?.
   admit.
-(* BNZ *)
-  + move=> im μ σ pc n m K r r1 j LPC rpcl -> ? get_r1 [<-] ?.
-    admit.
   (* PSetOff *)
   + move=> im μ σ pc fp' j K1 n K2 r r' r1 r2 r3 j' LPC rl rpcl -> ? get_r1 get_r2 [<- <-].
     rewrite /Vector.nth_order /= => upd_r3.
